examples/elliptic/arm/mlton/bsubstML.sml
@@ -57,46 +57,46 @@ struct
   fun mem_items m = Redblackmap.listItems m
  
   fun ADDR30 addr =
-        word_extract_itself (Tyop ("i30", [])) (fromString"31") TWO addr
+        word_extract_itself (Tyop ("30", [])) (fromString"31") TWO addr
     
   fun GET_HALF oareg data =
         if index oareg ONE
-          then word_extract_itself (Tyop ("i16", [])) (fromString"31")
+          then word_extract_itself (Tyop ("16", [])) (fromString"31")
                  (fromString"16") data
-          else word_extract_itself (Tyop ("i16", [])) (fromString"15")
+          else word_extract_itself (Tyop ("16", [])) (fromString"15")
                  ZERO data
     
   fun GET_BYTE oareg data =
-        case word_eq oareg (n2w_itself (ZERO,(Tyop ("i2", []))))
+        case word_eq oareg (n2w_itself (ZERO,(Tyop ("2", []))))
          of true =>
-               word_extract_itself (Tyop ("i8", [])) (fromString"7")
-                 ZERO data
+               word_extract_itself (Tyop ("8", [])) (fromString"7") ZERO
+                 data
           | false =>
-               (case word_eq oareg (n2w_itself (ONE,(Tyop ("i2", []))))
+               (case word_eq oareg (n2w_itself (ONE,(Tyop ("2", []))))
                 of true =>
-                      word_extract_itself (Tyop ("i8", []))
+                      word_extract_itself (Tyop ("8", []))
                         (fromString"15") (fromString"8") data
                  | false =>
                       (case
                          word_eq oareg
-                           (n2w_itself (TWO,(Tyop ("i2", []))))
+                           (n2w_itself (TWO,(Tyop ("2", []))))
                        of true =>
-                             word_extract_itself (Tyop ("i8", []))
+                             word_extract_itself (Tyop ("8", []))
                                (fromString"23") (fromString"16") data
                         | false =>
-                             word_extract_itself (Tyop ("i8", []))
+                             word_extract_itself (Tyop ("8", []))
                                (fromString"31") (fromString"24") data))
     
   fun FORMAT fmt oareg data =
         case fmt
          of SignedByte =>
-               sw2sw_itself (Tyop ("i32", [])) (GET_BYTE oareg data)
+               sw2sw_itself (Tyop ("32", [])) (GET_BYTE oareg data)
           | UnsignedByte =>
-               w2w_itself (Tyop ("i32", [])) (GET_BYTE oareg data)
+               w2w_itself (Tyop ("32", [])) (GET_BYTE oareg data)
           | SignedHalfWord =>
-               sw2sw_itself (Tyop ("i32", [])) (GET_HALF oareg data)
+               sw2sw_itself (Tyop ("32", [])) (GET_HALF oareg data)
           | UnsignedHalfWord =>
-               w2w_itself (Tyop ("i32", [])) (GET_HALF oareg data)
+               w2w_itself (Tyop ("32", [])) (GET_HALF oareg data)
           | UnsignedWord =>
                word_ror data ( *  (fromString"8") (w2n oareg))
     
@@ -104,23 +104,23 @@ struct
         word_modify (fn i => fn x =>
           < i (fromString"8")
           andalso
-          (if word_eq oareg (n2w_itself (ZERO,(Tyop ("i2", []))))
+          (if word_eq oareg (n2w_itself (ZERO,(Tyop ("2", []))))
              then index b i else x)
           orelse
           ((<= (fromString"8") i andalso < i (fromString"16"))
            andalso
-           (if word_eq oareg (n2w_itself (ONE,(Tyop ("i2", []))))
+           (if word_eq oareg (n2w_itself (ONE,(Tyop ("2", []))))
               then index b (- i (fromString"8")) else x)
            orelse
            ((<= (fromString"16") i andalso < i (fromString"24"))
             andalso
-            (if word_eq oareg (n2w_itself (TWO,(Tyop ("i2", []))))
+            (if word_eq oareg (n2w_itself (TWO,(Tyop ("2", []))))
                then index b (- i (fromString"16")) else x)
             orelse
             (<= (fromString"24") i andalso < i (fromString"32"))
             andalso
             (if word_eq oareg
-                  (n2w_itself ((fromString"3"),(Tyop ("i2", []))))
+                  (n2w_itself ((fromString"3"),(Tyop ("2", []))))
                then index b (- i (fromString"24")) else x)))) w
     
   fun SET_HALF oareg hw w =
@@ -138,7 +138,7 @@ struct
         in
            mem_write mem addr30
              (SET_BYTE
-                (word_extract_itself (Tyop ("i2", [])) ONE ZERO addr)
+                (word_extract_itself (Tyop ("2", [])) ONE ZERO addr)
                 word (mem_read (mem,addr30)))
         end
     
