examples/elliptic/arm/bsubstScript.sml
@@ -57,84 +57,6 @@ val _ = computeLib.auto_import_definitions := true;
 
 (* ------------------------------------------------------------------------- *)
 
-val _ = Hol_datatype
-  `formats = SignedByte | UnsignedByte
-           | SignedHalfWord | UnsignedHalfWord
-           | UnsignedWord`;
-
-val _ = Hol_datatype
-  `data = Byte of word8 | Half of word16 | Word of word32`;
-
-val _ = type_abbrev("mem", ``:word30->word32``);
-
-val GET_BYTE_def = Define`
-  GET_BYTE (oareg:word2) (data:word32) =
-    (case oareg of
-        0w -> (7 >< 0) data
-     || 1w -> (15 >< 8) data
-     || 2w -> (23 >< 16) data
-     || _  -> (31 >< 24) data):word8`;
-
-val GET_HALF_def = Define`
-  GET_HALF (oareg:word2) (data:word32) =
-    (if oareg %% 1 then
-       (31 >< 16) data
-     else
-       (15 >< 0) data):word16`;
-
-val FORMAT_def = Define`
-  FORMAT fmt oareg data =
-    case fmt of
-       SignedByte       -> sw2sw (GET_BYTE oareg data)
-    || UnsignedByte     -> w2w (GET_BYTE oareg data)
-    || SignedHalfWord   -> sw2sw (GET_HALF oareg data)
-    || UnsignedHalfWord -> w2w (GET_HALF oareg data)
-    || UnsignedWord     -> data #>> (8 * w2n oareg)`;
-
-val SET_BYTE_def = Define`
-  SET_BYTE (oareg:word2) (b:word8) (w:word32) =
-    word_modify (\i x.
-                  (i < 8) /\ (if oareg = 0w then b %% i else x) \/
-       (8 <= i /\ i < 16) /\ (if oareg = 1w then b %% (i - 8) else x) \/
-      (16 <= i /\ i < 24) /\ (if oareg = 2w then b %% (i - 16) else x) \/
-      (24 <= i /\ i < 32) /\ (if oareg = 3w then b %% (i - 24) else x)) w`;
-
-val SET_HALF_def = Define`
-  SET_HALF (oareg:bool) (hw:word16) (w:word32) =
-    word_modify (\i x.
-                 (i < 16) /\ (if ~oareg then hw %% i else x) \/
-      (16 <= i /\ i < 32) /\ (if oareg then hw %% (i - 16) else x)) w`;
-
-val ADDR30_def = Define `ADDR30 (addr:word32) = (31 >< 2) addr:word30`;
-
-val MEM_WRITE_BYTE_def = Define`
-  MEM_WRITE_BYTE (mem:mem) addr (word:word8) =
-    let addr30 = ADDR30 addr in
-      (addr30 :- SET_BYTE ((1 >< 0) addr) word (mem addr30)) mem`;
-
-val MEM_WRITE_HALF_def = Define`
-  MEM_WRITE_HALF (mem:mem) addr (word:word16) =
-    let addr30 = ADDR30 addr in
-      (addr30 :- SET_HALF (addr %% 1) word (mem addr30)) mem`;
-
-val MEM_WRITE_WORD_def = Define`
-  MEM_WRITE_WORD (mem:mem) addr word = (ADDR30 addr :- word) mem`;
-
-val MEM_WRITE_def = Define`
-  MEM_WRITE mem addr d =
-    case d of
-       Byte b  -> MEM_WRITE_BYTE mem addr b
-    || Half hw -> MEM_WRITE_HALF mem addr hw
-    || Word w  -> MEM_WRITE_WORD mem addr w`;
-
-val mem_read_def        = Define`mem_read (m: mem, a) = m a`;
-val mem_write_def       = Define`mem_write (m:mem) a d = (a :- d) m`;
-val mem_write_block_def = Define`mem_write_block (m:mem) a c = (a ::- c) m`;
-val mem_items_def       = Define`mem_items (m:mem) = []:(word30 # word32) list`;
-val empty_memory_def    = Define`empty_memory = (\a. 0xE6000010w):mem`;
-
-(* ------------------------------------------------------------------------- *)
-
 val JOIN_lem = prove(`!a b. MAX (SUC a) (SUC b) = SUC (MAX a b)`,
    RW_TAC std_ss [MAX_DEF]);
 
@@ -222,51 +144,6 @@ val BSUBST_BSUBST = store_thm("BSUBST_BSUBST",
             \\ IMP_RES_TAC LENGTH_NIL
             \\ RW_TAC (arith_ss++boolSimps.LET_ss) [WORD_LS,BSUBST_def]
             \\ FULL_SIMP_TAC arith_ss []]]);
-
-(* ------------------------------------------------------------------------- *)
-
-val RHS_REWRITE_RULE =
-  GEN_REWRITE_RULE (DEPTH_CONV o RAND_CONV) empty_rewrites;
-
-val defs_rule =
-  BETA_RULE o PURE_REWRITE_RULE
-    [GSYM n2w_itself_def, GSYM w2w_itself_def, GSYM sw2sw_itself_def,
-     GSYM word_extract_itself_def,GSYM mem_write_def] o
-  RHS_REWRITE_RULE [GSYM word_eq_def] o
-  ONCE_REWRITE_RULE [GSYM mem_read_def];
-
-val _ = ConstMapML.insert ``dimword``;
-val _ = ConstMapML.insert ``dimindex``;
-val _ = ConstMapML.insert ``INT_MIN``;
-val _ = ConstMapML.insert ``n2w_itself``;
-
-val _ = let open EmitML in emitML (!Globals.emitMLDir)
-    ("bsubst", OPEN ["num", "fcp", "words"]
-         :: MLSIG "type 'a word = 'a wordsML.word"
-         :: MLSIG "type num = numML.num"
-         :: MLSIG "type word2 = wordsML.word2"
-         :: MLSIG "type word8 = wordsML.word8"
-         :: MLSIG "type word16 = wordsML.word16"
-         :: MLSIG "type word30 = wordsML.word30"
-         :: MLSIG "type word32 = wordsML.word32"
-         :: MLSTRUCT "type mem = word30->word32"
-         :: MLSIG "type mem"
-         :: MLSTRUCT "val mem_updates = ref ([]: word30 list)"
-         :: MLSIG "val mem_updates : word30 list ref"
-         :: DATATYPE (`formats = SignedByte | UnsignedByte
-                               | SignedHalfWord | UnsignedHalfWord
-                               | UnsignedWord`)
-         :: DATATYPE (`data = Byte of word8 | Half of word16 | Word of word32`)
-         :: map DEFN
-              [SUBST_def, BSUBST_def, mem_read_def,
-               mem_write_def,  mem_write_block_def]
-          @ map (DEFN o defs_rule)
-              [empty_memory_def, mem_items_def, ADDR30_def, GET_HALF_def,
-               SIMP_RULE std_ss [literal_case_DEF] GET_BYTE_def,
-               FORMAT_def, SET_BYTE_def, SET_HALF_def,
-               MEM_WRITE_BYTE_def, MEM_WRITE_HALF_def,
-               MEM_WRITE_WORD_def, MEM_WRITE_def])
-end;
 
 (* ------------------------------------------------------------------------- *)
 
