examples/elliptic/arm/systemScript.sml
@@ -1,0 +1,1174 @@
+(* ========================================================================= *)
+(* FILE          : systemScript.sml                                          *)
+(* DESCRIPTION   : Model of a basic ARM system, with upto 16 coprocessors    *)
+(*                 plus main memory.                                         *)
+(* AUTHOR        : Anthony Fox (with some contributions by Juliano Iyoda)    *)
+(*                 University of Cambridge                                   *)
+(* DATE          : 2005 - 2006                                               *)
+(* ========================================================================= *)
+
+(* interactive use: 
+  app load ["wordsLib","wordsSyntax","armTheory"];
+*)
+
+open HolKernel boolLib bossLib Parse;
+open Q wordsTheory rich_listTheory bsubstTheory;
+open armTheory;
+
+val _ = new_theory "system";
+
+(* -------------------------------------------------------------------------- *)
+(* In what follows, the term "cp" stands for "coprocessor".                   *)
+(* -------------------------------------------------------------------------- *)
+
+(* -------------------------------------------------------------------------- *)
+(* We assume that there are up to 16 coprocessor with 16 registers each.      *)
+(* The register word size can be different for each coprocessor               *)
+(* -------------------------------------------------------------------------- *)
+
+val _ = Hol_datatype `cp_register = c0   | c1   | c2   | c3
+                                  | c4   | c5   | c6   | c7
+                                  | c8   | c9   | c10  | c11
+                                  | c12  | c13  | c14  | c15`;
+
+val _ = type_abbrev("cp_registers",``:cp_register->'a word``);
+
+val _ = Hol_datatype`
+  all_cp_registers =
+    <| p0_registers:'a0 cp_registers;
+       p1_registers:'a1 cp_registers;
+       p2_registers:'a2 cp_registers;
+       p3_registers:'a3 cp_registers;
+       p4_registers:'a4 cp_registers;
+       p5_registers:'a5 cp_registers;
+       p6_registers:'a6 cp_registers;
+       p7_registers:'a7 cp_registers;
+       p8_registers:'a8 cp_registers;
+       p9_registers:'a9 cp_registers;
+       p10_registers:'a10 cp_registers;
+       p11_registers:'a11 cp_registers;
+       p12_registers:'a12 cp_registers;
+       p13_registers:'a13 cp_registers;
+       p14_registers:'a14 cp_registers;
+       p15_registers:32 cp_registers
+    |>`;
+
+(* -------------------------------------------------------------------------- *)
+(* Memory + CP and bus output                                                 *)
+(* -------------------------------------------------------------------------- *)
+
+val _ = type_abbrev("mem", ``:word30->word32``);
+
+val _ = Hol_datatype`
+  cp_output = <| data : word32 option list; absent : bool |>`;
+
+val _ = Hol_datatype`
+  bus = <| data : word32 list; memory : mem; abort : num option;
+           p15_registers : 32 cp_registers |>`;
+
+(* -------------------------------------------------------------------------- *)
+(* The system state                                                           *)
+(* -------------------------------------------------------------------------- *)
+
+val _ = Hol_datatype`
+  arm_sys_state =
+     <| registers : registers;
+        psrs : psrs;
+        memory : mem;
+        undefined : bool;
+        cp_registers : ('a0,'a1,'a2,'a3,'a4,'a5,'a6,'a7,
+                        'a8,'a9,'a10,'a11,'a12,'a13,'a14) all_cp_registers
+     |>`;
+
+val Rg = inst [alpha |-> ``:32``,beta |-> ``:4``] wordsSyntax.word_extract_tm;
+
+(* -------------------------------------------------------------------------- *)
+(* The model is paramaterised by a collection of coprocessor operations       *)
+(* i.e. sixteen mrc, mcr, stc, ldc and cdp functions:                         *)
+(*                                                                            *)
+(* absent : user_mode ireg => bool                                            *)
+(*                                - controls which instructions are accepted  *)
+(* f_mrc : user_mode regs Cop1 Cop2 CRn CRm => word32                         *)
+(*                                - output for MRC instruction                *)
+(* f_mcr : user_mode regs Cop1 Cop2 data CRm => regs                          *)
+(*                                - operation for MCR instruction             *)
+(* f_stc : user_mode regs N CRd => word32 option list                         *)
+(*                                - output for STC instruction                *)
+(* f_ldc : user_mode regs N CRd data => regs                                  *)
+(*                                - operation for LDC instruction             *)
+(* f_cdp : user_mode regs Cop1 Cop2 CRd CRn CRm => regs                       *)
+(*                                - operation for CDP instruction             *)
+(* -------------------------------------------------------------------------- *)
+
+val _ = Hol_datatype `coproc_ops =
+  <| absent:bool->word32->bool;
+     f_mrc:bool->'a cp_registers->word3->word3->word4->word4->word32;
+     f_mcr:bool->'a cp_registers->word3->word3-> word32->word4->'a cp_registers;
+     f_stc:bool->'a cp_registers->bool->word4->word32 option list;
+     f_ldc:bool->'a cp_registers->word4->bool->word32 list->'a cp_registers;
+     f_cdp:bool->'a cp_registers->word4->word3->
+           word4->word4->word4->'a cp_registers
+  |>`;
+
+val _ = Hol_datatype `all_coproc_ops =
+  <| p0_ops : 'a0 coproc_ops;
+     p1_ops : 'a1 coproc_ops;
+     p2_ops : 'a2 coproc_ops;
+     p3_ops : 'a3 coproc_ops;
+     p4_ops : 'a4 coproc_ops;
+     p5_ops : 'a5 coproc_ops;
+     p6_ops : 'a6 coproc_ops;
+     p7_ops : 'a7 coproc_ops;
+     p8_ops : 'a8 coproc_ops;
+     p9_ops : 'a9 coproc_ops;
+     p10_ops : 'a10 coproc_ops;
+     p11_ops : 'a11 coproc_ops;
+     p12_ops : 'a12 coproc_ops;
+     p13_ops : 'a13 coproc_ops;
+     p14_ops : 'a14 coproc_ops;
+     p15_ops : 32 coproc_ops
+  |>`;
+
+(* -------------------------------------------------------------------------- *)
+(* REG_READ_CP and REG_WRITE_CP                                               *)
+(* -------------------------------------------------------------------------- *)
+
+val word2cp_register = Define`
+  word2cp_register (n:word4) = num2cp_register (w2n n)`;
+
+val CP_REG_READ_def = Define`
+  CP_REG_READ (cp_registers:'a cp_registers) n =
+    cp_registers (word2cp_register n)`;
+
+val CP_REG_WRITE_def = Define`
+  CP_REG_WRITE (cp_registers:'a cp_registers) n data =
+    ((word2cp_register n :- data) cp_registers)`;
+
+(* -------------------------------------------------------------------------- *)
+(* DECODE_CDP                                                                 *)
+(* -------------------------------------------------------------------------- *)
+
+val DECODE_CDP_def = Define`
+  DECODE_CDP (ireg:word32) =
+    (^Rg 23 20 ireg,          (* Cop1 *)
+     ^Rg 19 16 ireg,          (* CRn *)
+     ^Rg 15 12 ireg,          (* CRd *)
+     ((7 >< 5) ireg):word3, (* Cop2 *)
+     ^Rg 03 00 ireg)`;        (* CRm *)
+
+(* -------------------------------------------------------------------------- *)
+(* DECODE_MRC_MCR                                                             *)
+(* -------------------------------------------------------------------------- *)
+
+val DECODE_MRC_MCR_def = Define`
+  DECODE_MRC_MCR (ireg:word32) =
+    (((23 >< 21) ireg):word3, (* Cop1 *)
+     ^Rg 19 16 ireg,          (* CRn *)
+     ((07 >< 05) ireg):word3, (* Cop2 *)
+     ^Rg 03 00 ireg)`;        (* CRm *)
+
+(* -------------------------------------------------------------------------- *)
+(* DECODE_LDC_STC'                                                            *)
+(* -------------------------------------------------------------------------- *)
+
+val DECODE_LDC_STC'_def = Define`
+  DECODE_LDC_STC' w =
+    (w %% 22,               (* N *)
+     ^Rg 15 12 w)`;         (* CRd *)
+
+(* -------------------------------------------------------------------------- *)
+(* CP                                                                         *)
+(* Returns the coprocessor number from the instruction                        *)
+(* -------------------------------------------------------------------------- *)
+
+val CP_def = Define `CP (w:word32) = ((11 >< 8) w):word4`;
+
+(* -------------------------------------------------------------------------- *)
+(* DECODE_CP                                                                  *)
+(* Determines the instruction class ** for a coprocessor instruction **       *)
+(* -------------------------------------------------------------------------- *)
+
+val DECODE_CP_def = Define`
+  DECODE_CP (w:word32) =
+    case ((26 >< 25) w):word3 of
+       6w -> ldc_stc
+    || 7w -> if ~(w %% 24) /\ w %% 4 then
+               if w %% 20 then mrc else mcr
+             else
+               cdp_und
+    || _ -> cdp_und`;
+
+(* -------------------------------------------------------------------------- *)
+(* MRC_OUT                                                                    *)
+(* -------------------------------------------------------------------------- *)
+
+val MRC_OUT_def = Define`
+  MRC_OUT f_mrc (cp_registers:'a cp_registers) ireg user_mode =
+    let (Cop1,CRn,Cop2,CRm) = DECODE_MRC_MCR ireg
+    in
+      [SOME (f_mrc user_mode cp_registers Cop1 Cop2 CRn CRm) ;
+       NONE: word32 option]`;
+
+(* -------------------------------------------------------------------------- *)
+(* STC_OUT                                                                    *)
+(* -------------------------------------------------------------------------- *)
+
+val STC_OUT_def = Define`
+  STC_OUT f_stc (cp_registers:'a cp_registers) ireg user_mode =
+    let (N,CRd) = DECODE_LDC_STC' ireg
+    in
+      (f_stc user_mode cp_registers N CRd):word32 option list`;
+
+(* -------------------------------------------------------------------------- *)
+(* OUT_CPN                                                                    *)
+(* Returns output from one coprocessor                                        *)
+(* -------------------------------------------------------------------------- *)
+
+val OUT_CPN_def = Define`
+  OUT_CPN cp_ops cp_registers ireg user_mode =
+    if cp_ops.absent user_mode ireg then
+      <| data := []; absent := T |>
+    else
+      <| data :=
+            case DECODE_CP ireg of
+               mrc     -> MRC_OUT cp_ops.f_mrc cp_registers ireg user_mode
+            || ldc_stc -> if ireg %% 20 then
+                            []
+                          else
+                            STC_OUT cp_ops.f_stc cp_registers ireg user_mode
+            || _ -> [];
+         absent := F |>`;
+                   
+(* -------------------------------------------------------------------------- *)
+(* OUT_CP                                                                     *)
+(* It is assumed that only one coprocessor (i.e. "CP ireg") can accept the    *)
+(* instruction but in general this need not be the case                       *)
+(* -------------------------------------------------------------------------- *)
+
+val OUT_CP_def = Define`
+  OUT_CP cp_ops cp_state ireg arm_out =
+    if arm_out.cpi then
+      case CP ireg of
+         0w  -> OUT_CPN cp_ops.p0_ops cp_state.p0_registers ireg arm_out.user
+      || 1w  -> OUT_CPN cp_ops.p1_ops cp_state.p1_registers ireg arm_out.user
+      || 2w  -> OUT_CPN cp_ops.p2_ops cp_state.p2_registers ireg arm_out.user
+      || 3w  -> OUT_CPN cp_ops.p3_ops cp_state.p3_registers ireg arm_out.user
+      || 4w  -> OUT_CPN cp_ops.p4_ops cp_state.p4_registers ireg arm_out.user
+      || 5w  -> OUT_CPN cp_ops.p5_ops cp_state.p5_registers ireg arm_out.user
+      || 6w  -> OUT_CPN cp_ops.p6_ops cp_state.p6_registers ireg arm_out.user
+      || 7w  -> OUT_CPN cp_ops.p7_ops cp_state.p7_registers ireg arm_out.user
+      || 8w  -> OUT_CPN cp_ops.p8_ops cp_state.p8_registers ireg arm_out.user
+      || 9w  -> OUT_CPN cp_ops.p9_ops cp_state.p9_registers ireg arm_out.user
+      || 10w -> OUT_CPN cp_ops.p10_ops cp_state.p10_registers ireg arm_out.user
+      || 11w -> OUT_CPN cp_ops.p11_ops cp_state.p11_registers ireg arm_out.user
+      || 12w -> OUT_CPN cp_ops.p12_ops cp_state.p12_registers ireg arm_out.user
+      || 13w -> OUT_CPN cp_ops.p13_ops cp_state.p13_registers ireg arm_out.user
+      || 14w -> OUT_CPN cp_ops.p14_ops cp_state.p14_registers ireg arm_out.user
+      || _   -> OUT_CPN cp_ops.p15_ops cp_state.p15_registers ireg arm_out.user
+    else <| data := []; absent := T |>`;
+
+
+(* -------------------------------------------------------------------------- *)
+(* MCR                                                                        *)
+(* -------------------------------------------------------------------------- *)
+
+val MCR_def = Define`
+  MCR f_mcr (cp_registers:'a cp_registers) (data:word32 list) ireg user_mode =
+    let (Cop1,CRn,Cop2,CRm) = DECODE_MRC_MCR ireg
+    in
+      f_mcr user_mode cp_registers Cop1 Cop2 (HD data) CRm`;
+
+(* -------------------------------------------------------------------------- *)
+(* LDC                                                                        *)
+(* -------------------------------------------------------------------------- *)
+
+val LDC_def = Define`
+  LDC f_ldc (cp_registers:'a cp_registers) (data:word32 list) ireg user_mode =
+    let (N,CRd) = DECODE_LDC_STC' ireg
+    in
+      f_ldc user_mode cp_registers CRd N data`;
+
+(* -------------------------------------------------------------------------- *)
+(* CDP                                                                        *)
+(* -------------------------------------------------------------------------- *)
+
+val CDP_def = Define`
+  CDP f_cdp (cp_registers:'a cp_registers) ireg user_mode =
+    let (Cop1,CRn,CRd,Cop2,CRm) = DECODE_CDP ireg
+    in
+      f_cdp user_mode cp_registers Cop1 Cop2 CRd CRn CRm`;
+
+(* -------------------------------------------------------------------------- *)
+(* RUN_CPN                                                                    *)
+(* Updates state of one coprocessor                                           *)
+(* -------------------------------------------------------------------------- *)
+
+val RUN_CPN_def = Define`
+  RUN_CPN cp_ops cp_registers data ireg user_mode =
+    case DECODE_CP ireg of
+       mcr     -> MCR cp_ops.f_mcr cp_registers data ireg user_mode
+    || ldc_stc -> if ireg %% 20 then
+                    LDC cp_ops.f_ldc cp_registers data ireg user_mode
+                  else
+                    cp_registers
+    || cdp_und -> CDP cp_ops.f_cdp cp_registers ireg user_mode
+    || _ -> cp_registers`;
+
+(* -------------------------------------------------------------------------- *)
+(* RUN_CP                                                                     *)
+(* Takes a CP state and the input (word32 list) and returns the next state    *)
+(* -------------------------------------------------------------------------- *)
+
+val RUN_CP_def = Define`
+  RUN_CP cp_ops cp_state absent data ireg arm_out =
+    if arm_out.cpi /\ ~absent then
+      case CP ireg of
+         0w  -> cp_state with p0_registers :=
+            RUN_CPN cp_ops.p0_ops cp_state.p0_registers data ireg arm_out.user
+      || 1w  -> cp_state with p1_registers :=
+            RUN_CPN cp_ops.p1_ops cp_state.p1_registers data ireg arm_out.user
+      || 2w  -> cp_state with p2_registers :=
+            RUN_CPN cp_ops.p2_ops cp_state.p2_registers data ireg arm_out.user
+      || 3w  -> cp_state with p3_registers :=
+            RUN_CPN cp_ops.p3_ops cp_state.p3_registers data ireg arm_out.user
+      || 4w  -> cp_state with p4_registers :=
+            RUN_CPN cp_ops.p4_ops cp_state.p4_registers data ireg arm_out.user
+      || 5w  -> cp_state with p5_registers :=
+            RUN_CPN cp_ops.p5_ops cp_state.p5_registers data ireg arm_out.user
+      || 6w  -> cp_state with p6_registers :=
+            RUN_CPN cp_ops.p6_ops cp_state.p6_registers data ireg arm_out.user
+      || 7w  -> cp_state with p7_registers :=
+            RUN_CPN cp_ops.p7_ops cp_state.p7_registers data ireg arm_out.user
+      || 8w  -> cp_state with p8_registers :=
+            RUN_CPN cp_ops.p8_ops cp_state.p8_registers data ireg arm_out.user
+      || 9w  -> cp_state with p9_registers :=
+            RUN_CPN cp_ops.p9_ops cp_state.p9_registers data ireg arm_out.user
+      || 10w -> cp_state with p10_registers :=
+            RUN_CPN cp_ops.p10_ops cp_state.p10_registers data ireg arm_out.user
+      || 11w -> cp_state with p11_registers :=
+            RUN_CPN cp_ops.p11_ops cp_state.p11_registers data ireg arm_out.user
+      || 12w -> cp_state with p12_registers :=
+            RUN_CPN cp_ops.p12_ops cp_state.p12_registers data ireg arm_out.user
+      || 13w -> cp_state with p13_registers :=
+            RUN_CPN cp_ops.p13_ops cp_state.p13_registers data ireg arm_out.user
+      || 14w -> cp_state with p14_registers :=
+            RUN_CPN cp_ops.p14_ops cp_state.p14_registers data ireg arm_out.user
+      || _   -> cp_state with p15_registers :=
+            RUN_CPN cp_ops.p15_ops cp_state.p15_registers data ireg arm_out.user
+    else cp_state`;
+
+(* -------------------------------------------------------------------------- *)
+(* NEXT_ARM_SYS and STATE_ARM_SYS                                             *)
+(* NB. Assumes that there are no prefetch aborts or hardware                  *)
+(*     interrupts (fiq, irq)                                                  *)
+(* -------------------------------------------------------------------------- *)
+
+val ADDR30_def = Define `ADDR30 (addr:word32) = (31 >< 2) addr:word30`;
+
+val NEXT_ARM_SYS_def = Define`
+  NEXT_ARM_SYS bus_op (cp_ops: ('a0,'a1,'a2,'a3,'a4,'a5,'a6,'a7,
+                         'a8,'a9,'a10,'a11,'a12,'a13,'a14) all_coproc_ops)
+          state =
+    let ireg = state.memory (ADDR30 (FETCH_PC state.registers)) in
+    let s = <| regs := <| reg := state.registers; psr := state.psrs |>;
+               ireg := ireg;
+               exception := if state.undefined then undefined else software |>
+    in
+    let arm_out = OUT_ARM s
+    in
+    let cp_out  = OUT_CP cp_ops state.cp_registers ireg arm_out
+    in
+    let bus = bus_op arm_out state.cp_registers.p15_registers
+                      cp_out.data state.memory
+    in
+    let r = RUN_ARM s (if IS_SOME bus.abort then
+                          SOME (THE bus.abort)
+                       else
+                          NONE)
+                       bus.data cp_out.absent
+    and p = RUN_CP cp_ops
+                   (state.cp_registers with
+                      p15_registers := bus.p15_registers)
+                   cp_out.absent bus.data ireg arm_out
+    in
+      <| registers := r.reg; psrs := r.psr; memory := bus.memory;
+         undefined := (~state.undefined /\ arm_out.cpi /\ cp_out.absent);
+         cp_registers := p |>`;
+
+val STATE_ARM_SYS_def = Define`
+  (STATE_ARM_SYS bus_op co_ops 0 s = s) /\
+  (STATE_ARM_SYS bus_op co_ops (SUC t) s =
+    NEXT_ARM_SYS bus_op co_ops (STATE_ARM_SYS bus_op co_ops t s))`;
+
+(* -------------------------------------------------------------------------- *)
+(* An Idealistic Memory Model                                                 *)
+(* -------------------------------------------------------------------------- *)
+
+val SET_BYTE_def = Define`
+  SET_BYTE (oareg:word2) (b:word8) (w:word32) =
+    word_modify (\i x.
+                  (i < 8) /\ (if oareg = 0w then b %% i else x) \/
+       (8 <= i /\ i < 16) /\ (if oareg = 1w then b %% (i - 8) else x) \/
+      (16 <= i /\ i < 24) /\ (if oareg = 2w then b %% (i - 16) else x) \/
+      (24 <= i /\ i < 32) /\ (if oareg = 3w then b %% (i - 24) else x)) w`;
+
+val SET_HALF_def = Define`
+  SET_HALF (oareg:bool) (hw:word16) (w:word32) =
+    word_modify (\i x.
+                 (i < 16) /\ (if ~oareg then hw %% i else x) \/
+      (16 <= i /\ i < 32) /\ (if oareg then hw %% (i - 16) else x)) w`;
+
+val MEM_WRITE_BYTE_def = Define`
+  MEM_WRITE_BYTE (mem:mem) addr (word:word8) =
+    let addr30 = ADDR30 addr in
+      (addr30 :- SET_BYTE ((1 >< 0) addr) word (mem addr30)) mem`;
+
+val MEM_WRITE_HALF_def = Define`
+  MEM_WRITE_HALF (mem:mem) addr (word:word16) =
+    let addr30 = ADDR30 addr in
+      (addr30 :- SET_HALF (addr %% 1) word (mem addr30)) mem`;
+
+val MEM_WRITE_WORD_def = Define`
+  MEM_WRITE_WORD (mem:mem) addr word = (ADDR30 addr :- word) mem`;
+
+val MEM_WRITE_def = Define`
+  MEM_WRITE mem addr d =
+    case d of
+       Byte b  -> MEM_WRITE_BYTE mem addr b
+    || Half hw -> MEM_WRITE_HALF mem addr hw
+    || Word w  -> MEM_WRITE_WORD mem addr w`;
+
+val TRANSFER_def = Define`
+  TRANSFER cpi (cp_data,data,mem) t =
+    case t of
+       MemRead a ->
+         if cpi then
+           let (f, b) = SPLITP IS_SOME cp_data in
+             (b, data ++
+                MAP (\addr. mem (ADDR30 addr)) (ADDRESS_LIST a (LENGTH f)), mem)
+         else
+           (cp_data, data ++ [mem (ADDR30 a)], mem)
+    || MemWrite a d ->
+         if cpi then
+           let (f, b) = SPLITP IS_NONE cp_data in
+             (b, data,
+                FOLDL (\m (addr,cpd). MEM_WRITE mem addr (Word (THE cpd)))
+                  mem (ZIP (ADDRESS_LIST a (LENGTH f), f)))
+         else
+            (cp_data, data, MEM_WRITE mem a d)
+    || CPWrite w ->
+         (cp_data, if cpi then data ++ [w] else data, mem)`;
+
+val TRANSFERS_def = Define`
+  TRANSFERS arm_out p15_regs cp_data mem =
+    let (data, mem) = 
+      if arm_out.cpi /\ NULL arm_out.transfers then
+        (MAP THE cp_data, mem)
+      else
+        SND (FOLDL (TRANSFER arm_out.cpi) (cp_data, [], mem) arm_out.transfers)
+    in
+      <| data := data; memory := mem;
+         abort := NONE; p15_registers := p15_regs |>`;
+
+(* -------------------------------------------------------------------------- *)
+(* NEXT_ARM_MEM and STATE_ARM_MEM                                             *)
+(* -------------------------------------------------------------------------- *)
+
+val NO_CP_OPS_def = Define`
+  NO_CP_OPS = <|
+    p0_ops  := <| absent := \u i. T; f_mrc := ARB; f_mcr := ARB;
+                   f_stc := ARB; f_ldc := ARB; f_cdp := ARB |>;
+    p1_ops  := <| absent := \u i. T; f_mrc := ARB; f_mcr := ARB;
+                   f_stc := ARB; f_ldc := ARB; f_cdp := ARB |>;
+    p2_ops  := <| absent := \u i. T; f_mrc := ARB; f_mcr := ARB;
+                   f_stc := ARB; f_ldc := ARB; f_cdp := ARB |>;
+    p3_ops  := <| absent := \u i. T; f_mrc := ARB; f_mcr := ARB;
+                   f_stc := ARB; f_ldc := ARB; f_cdp := ARB |>;
+    p4_ops  := <| absent := \u i. T; f_mrc := ARB; f_mcr := ARB;
+                   f_stc := ARB; f_ldc := ARB; f_cdp := ARB |>;
+    p5_ops  := <| absent := \u i. T; f_mrc := ARB; f_mcr := ARB;
+                   f_stc := ARB; f_ldc := ARB; f_cdp := ARB |>;
+    p6_ops  := <| absent := \u i. T; f_mrc := ARB; f_mcr := ARB;
+                   f_stc := ARB; f_ldc := ARB; f_cdp := ARB |>;
+    p7_ops  := <| absent := \u i. T; f_mrc := ARB; f_mcr := ARB;
+                   f_stc := ARB; f_ldc := ARB; f_cdp := ARB |>;
+    p8_ops  := <| absent := \u i. T; f_mrc := ARB; f_mcr := ARB;
+                   f_stc := ARB; f_ldc := ARB; f_cdp := ARB |>;
+    p9_ops  := <| absent := \u i. T; f_mrc := ARB; f_mcr := ARB;
+                   f_stc := ARB; f_ldc := ARB; f_cdp := ARB |>;
+    p10_ops := <| absent := \u i. T; f_mrc := ARB; f_mcr := ARB;
+                   f_stc := ARB; f_ldc := ARB; f_cdp := ARB |>;
+    p11_ops := <| absent := \u i. T; f_mrc := ARB; f_mcr := ARB;
+                   f_stc := ARB; f_ldc := ARB; f_cdp := ARB |>;
+    p12_ops := <| absent := \u i. T; f_mrc := ARB; f_mcr := ARB;
+                   f_stc := ARB; f_ldc := ARB; f_cdp := ARB |>;
+    p13_ops := <| absent := \u i. T; f_mrc := ARB; f_mcr := ARB;
+                   f_stc := ARB; f_ldc := ARB; f_cdp := ARB |>;
+    p14_ops := <| absent := \u i. T; f_mrc := ARB; f_mcr := ARB;
+                   f_stc := ARB; f_ldc := ARB; f_cdp := ARB |>;
+    p15_ops := <| absent := \u i. T; f_mrc := ARB; f_mcr := ARB;
+                   f_stc := ARB; f_ldc := ARB; f_cdp := ARB |>
+  |>`;
+
+val OUT_CP_NO_CPS =
+  SIMP_CONV (srw_ss()) [OUT_CP_def,OUT_CPN_def,NO_CP_OPS_def,bool_case_EQ_COND]
+  ``OUT_CP NO_CP_OPS cp_state ireg arm_out``;
+
+val RUN_CP_NO_CPS = SIMP_CONV (srw_ss()) [RUN_CP_def,NO_CP_OPS_def]
+  ``RUN_CP NO_CP_OPS cp_state T data ireg arm_out``;
+
+val NEXT_ARM_MEM_def = Define `NEXT_ARM_MEM = NEXT_ARM_SYS TRANSFERS NO_CP_OPS`;
+
+val STATE_ARM_MEM_def = Define`
+  (STATE_ARM_MEM 0 s = s) /\
+  (STATE_ARM_MEM (SUC t) s = NEXT_ARM_MEM (STATE_ARM_MEM t s))`;
+
+infix \\ << >>
+
+val op \\ = op THEN;
+val op << = op THENL;
+val op >> = op THEN1;
+
+val TRANSFERS = prove(
+  `(!arm_out p15_reg data mem.
+        (TRANSFERS arm_out p15_reg data mem).abort = NONE) /\
+   (!arm_out p15_reg data mem.
+        (TRANSFERS arm_out p15_reg data mem).p15_registers = p15_reg)`,
+  SRW_TAC [] [TRANSFERS_def] \\ FULL_SIMP_TAC (srw_ss()) []);
+
+val NEXT_ARM_MEM = store_thm("NEXT_ARM_MEM",
+  `NEXT_ARM_MEM state =
+     let ireg = state.memory (ADDR30 (FETCH_PC state.registers)) in
+     let s = <| regs := <| reg := state.registers; psr := state.psrs |>;
+                ireg := ireg;
+                exception := if state.undefined then undefined else software |>
+     in
+     let arm_out = OUT_ARM s in
+     let mmu_out = TRANSFERS arm_out state.cp_registers.p15_registers []
+                             state.memory
+     in
+     let r = RUN_ARM s NONE mmu_out.data T
+     in
+       <| registers := r.reg; psrs := r.psr; memory := mmu_out.memory;
+          undefined := (~state.undefined /\ arm_out.cpi);
+          cp_registers := state.cp_registers |>`,
+  SRW_TAC [boolSimps.LET_ss]
+    [NEXT_ARM_SYS_def,NEXT_ARM_MEM_def,RUN_CP_NO_CPS,OUT_CP_NO_CPS,TRANSFERS]
+    \\ Cases_on `state.cp_registers`
+    \\ SIMP_TAC (srw_ss()) [definition "all_cp_registers_p15_registers_fupd"]);
+
+(* ------------------------------------------------------------------------- *)
+(* Export ML versions of functions                                           *)
+(*---------------------------------------------------------------------------*)
+
+val mem_read_def        = Define`mem_read (m: mem, a) = m a`;
+val mem_write_def       = Define`mem_write (m:mem) a d = (a :- d) m`;
+val mem_write_block_def = Define`mem_write_block (m:mem) a c = (a ::- c) m`;
+val mem_items_def       = Define`mem_items (m:mem) = []:(word30 # word32) list`;
+val empty_memory_def    = Define`empty_memory = (\a. 0xE6000010w):mem`;
+val empty_registers_def = Define`empty_registers = (\n. 0w):registers`;
+val empty_psrs_def      = Define`empty_psrs = (\x. SET_IFMODE F F usr 0w):psrs`;
+
+val empty_cp_registers_def = Define`
+  empty_cp_registers = (\n. 0w):one cp_registers`;
+
+val empty_all_cp_registers_def = Define`
+  empty_all_cp_registers =
+    <| p0_registers := empty_cp_registers;
+       p1_registers := empty_cp_registers;
+       p2_registers := empty_cp_registers;
+       p3_registers := empty_cp_registers;
+       p4_registers := empty_cp_registers;
+       p5_registers := empty_cp_registers;
+       p6_registers := empty_cp_registers;
+       p7_registers := empty_cp_registers;
+       p8_registers := empty_cp_registers;
+       p9_registers := empty_cp_registers;
+       p10_registers := empty_cp_registers;
+       p11_registers := empty_cp_registers;
+       p12_registers := empty_cp_registers;
+       p13_registers := empty_cp_registers;
+       p14_registers := empty_cp_registers;
+       p15_registers := (\n. 0w)
+    |>`;
+
+(* ------------------------------------------------------------------------- *)
+
+open arithmeticTheory numeralTheory bitTheory;
+
+val std_ss = std_ss ++ boolSimps.LET_ss;
+val arith_ss = arith_ss ++ boolSimps.LET_ss;
+
+val word_ss = arith_ss++fcpLib.FCP_ss++wordsLib.SIZES_ss++
+  rewrites [n2w_def,word_extract_def,word_bits_n2w,w2w,
+    BIT_def,BITS_THM,DIVMOD_2EXP_def,DIV_2EXP_def,DIV_1,
+    DIV2_def,ODD_MOD2_LEM,DIV_DIV_DIV_MULT,MOD_2EXP_def]
+
+val MOD_DIMINDEX_32 = (SIMP_RULE (std_ss++wordsLib.SIZES_ss) [] o
+   Thm.INST_TYPE [alpha |-> ``:32``]) MOD_DIMINDEX;
+
+val DECODE_TAC = SIMP_TAC std_ss [DECODE_PSR_def,DECODE_BRANCH_def,
+      DECODE_DATAP_def,DECODE_MRS_def,DECODE_MSR_def,DECODE_LDR_STR_def,
+      DECODE_LDRH_STRH_def,DECODE_MLA_MUL_def,DECODE_LDM_STM_def,
+      DECODE_SWP_def,DECODE_LDC_STC_def,SHIFT_IMMEDIATE_def,SHIFT_REGISTER_def,
+      CONV_RULE numLib.SUC_TO_NUMERAL_DEFN_CONV rich_listTheory.GENLIST,
+      NZCV_def,REGISTER_LIST_def,rich_listTheory.SNOC,word_extract_def]
+ \\ SIMP_TAC word_ss [];
+
+val DECODE_PSR_THM = store_thm("DECODE_PSR_THM",
+  `!n.  DECODE_PSR (n2w n) =
+     let (q0,m) = DIVMOD_2EXP 5 n in
+     let (q1,i) = DIVMOD_2EXP 1 (DIV2 q0) in
+     let (q2,f) = DIVMOD_2EXP 1 q1 in
+     let (q3,V) = DIVMOD_2EXP 1 (DIV_2EXP 20 q2) in
+     let (q4,C) = DIVMOD_2EXP 1 q3 in
+     let (q5,Z) = DIVMOD_2EXP 1 q4 in
+       ((ODD q5,Z=1,C=1,V=1),f = 1,i = 1,n2w m)`, DECODE_TAC);
+
+val DECODE_BRANCH_THM = store_thm("DECODE_BRANCH_THM",
+  `!n. DECODE_BRANCH (n2w n) =
+         let (L,offset) = DIVMOD_2EXP 24 n in (ODD L,n2w offset)`, DECODE_TAC);
+
+val DECODE_DATAP_THM = store_thm("DECODE_DATAP_THM",
+  `!n. DECODE_DATAP (n2w n) =
+     let (q0,opnd2) = DIVMOD_2EXP 12 n in
+     let (q1,Rd) = DIVMOD_2EXP 4 q0 in
+     let (q2,Rn) = DIVMOD_2EXP 4 q1 in
+     let (q3,S) = DIVMOD_2EXP 1 q2 in
+     let (q4,opcode) = DIVMOD_2EXP 4 q3 in
+       (ODD q4,n2w opcode,S = 1,n2w Rn,n2w Rd,n2w opnd2)`, DECODE_TAC);
+
+val DECODE_MRS_THM = store_thm("DECODE_MRS_THM",
+  `!n. DECODE_MRS (n2w n) =
+     let (q,Rd) = DIVMOD_2EXP 4 (DIV_2EXP 12 n) in
+      (ODD (DIV_2EXP 6 q),n2w Rd)`, DECODE_TAC);
+
+val DECODE_MSR_THM = store_thm("DECODE_MSR_THM",
+  `!n. DECODE_MSR (n2w n) =
+     let (q0,opnd) = DIVMOD_2EXP 12 n in
+     let (q1,bit16) = DIVMOD_2EXP 1 (DIV_2EXP 4 q0) in
+     let (q2,bit19) = DIVMOD_2EXP 1 (DIV_2EXP 2 q1) in
+     let (q3,R) = DIVMOD_2EXP 1 (DIV_2EXP 2 q2) in
+       (ODD (DIV_2EXP 2 q3),R = 1,bit19 = 1,bit16 = 1,
+        n2w (MOD_2EXP 4 opnd),n2w opnd)`,
+  DECODE_TAC \\ `4096 = 16 * 256` by numLib.ARITH_TAC
+    \\ ASM_REWRITE_TAC [] \\ SIMP_TAC arith_ss [MOD_MULT_MOD]);
+
+val DECODE_LDR_STR_THM = store_thm("DECODE_LDR_STR_THM",
+  `!n. DECODE_LDR_STR (n2w n) =
+    let (q0,offset) = DIVMOD_2EXP 12 n in
+    let (q1,Rd) = DIVMOD_2EXP 4 q0 in
+    let (q2,Rn) = DIVMOD_2EXP 4 q1 in
+    let (q3,L) = DIVMOD_2EXP 1 q2 in
+    let (q4,W) = DIVMOD_2EXP 1 q3 in
+    let (q5,B) = DIVMOD_2EXP 1 q4 in
+    let (q6,U) = DIVMOD_2EXP 1 q5 in
+    let (q7,P) = DIVMOD_2EXP 1 q6 in
+      (ODD q7,P = 1,U = 1,B = 1,W = 1,L = 1,n2w Rn,n2w Rd,n2w offset)`,
+   DECODE_TAC);
+
+val DECODE_LDRH_STRH_THM = store_thm("DECODE_LDRH_STRH_THM",
+  `!n. DECODE_LDRH_STRH (n2w n) =
+    let (q0,offsetL) = DIVMOD_2EXP 4 n in
+    let (q1,H) = DIVMOD_2EXP 1 (DIV2 q0) in
+    let (q2,S) = DIVMOD_2EXP 1 q1 in
+    let (q3,offsetH) = DIVMOD_2EXP 4 (DIV2 q2) in
+    let (q4,Rd) = DIVMOD_2EXP 4 q3 in
+    let (q5,Rn) = DIVMOD_2EXP 4 q4 in
+    let (q6,L) = DIVMOD_2EXP 1 q5 in
+    let (q7,W) = DIVMOD_2EXP 1 q6 in
+    let (q8,I) = DIVMOD_2EXP 1 q7 in
+    let (q9,U) = DIVMOD_2EXP 1 q8 in
+      (ODD q9,U = 1,I = 1,W = 1,L = 1,n2w Rn,n2w Rd,
+       n2w offsetH,S = 1,H = 1,n2w offsetL)`,
+   DECODE_TAC);
+
+val DECODE_MLA_MUL_THM = store_thm("DECODE_MLA_MUL_THM",
+  `!n. DECODE_MLA_MUL (n2w n) =
+    let (q0,Rm) = DIVMOD_2EXP 4 n in
+    let (q1,Rs) = DIVMOD_2EXP 4 (DIV_2EXP 4 q0) in
+    let (q2,Rn) = DIVMOD_2EXP 4 q1 in
+    let (q3,Rd) = DIVMOD_2EXP 4 q2 in
+    let (q4,S) = DIVMOD_2EXP 1 q3 in
+    let (q5,A) = DIVMOD_2EXP 1 q4 in
+    let (q6,Sgn) = DIVMOD_2EXP 1 q5 in
+      (ODD q6,Sgn = 1,A = 1,S = 1,n2w Rd,n2w Rn,n2w Rs,n2w Rm)`, DECODE_TAC);
+
+val DECODE_LDM_STM_THM = store_thm("DECODE_LDM_STM_THM",
+  `!n. DECODE_LDM_STM (n2w n) =
+    let (q0,list) = DIVMOD_2EXP 16 n in
+    let (q1,Rn) = DIVMOD_2EXP 4 q0 in
+    let (q2,L) = DIVMOD_2EXP 1 q1 in
+    let (q3,W) = DIVMOD_2EXP 1 q2 in
+    let (q4,S) = DIVMOD_2EXP 1 q3 in
+    let (q5,U) = DIVMOD_2EXP 1 q4 in
+      (ODD q5, U = 1, S = 1, W = 1, L = 1,n2w Rn,n2w list)`, DECODE_TAC);
+
+val DECODE_SWP_THM = store_thm("DECODE_SWP_THM",
+  `!n. DECODE_SWP (n2w n) =
+    let (q0,Rm) = DIVMOD_2EXP 4 n in
+    let (q1,Rd) = DIVMOD_2EXP 4 (DIV_2EXP 8 q0) in
+    let (q2,Rn) = DIVMOD_2EXP 4 q1 in
+      (ODD (DIV_2EXP 2 q2),n2w Rn,n2w Rd,n2w Rm)`, DECODE_TAC);
+
+val DECODE_LDC_STC_THM = store_thm("DECODE_LDC_STC_THM",
+  `!n. DECODE_LDC_STC (n2w n) =
+    let (q0,offset) = DIVMOD_2EXP 8 n in
+    let (q1,Rn) = DIVMOD_2EXP 4 (DIV_2EXP 8 q0) in
+    let (q2,L) = DIVMOD_2EXP 1 q1 in
+    let (q3,W) = DIVMOD_2EXP 1 q2 in
+    let (q4,U) = DIVMOD_2EXP 1 (DIV2 q3) in
+      (ODD q4,U = 1,W = 1,L = 1,n2w Rn,n2w offset)`, DECODE_TAC);
+
+(* ------------------------------------------------------------------------- *)
+
+fun w2w_n2w_sizes a b = (GSYM o SIMP_RULE (std_ss++wordsLib.SIZES_ss) [] o
+  Thm.INST_TYPE [alpha |-> a, beta |-> b]) w2w_n2w;
+
+val SHIFT_IMMEDIATE_THM = store_thm("SHIFT_IMMEDIATE_THM",
+  `!reg mode C opnd2.
+     SHIFT_IMMEDIATE reg mode C (n2w opnd2) =
+       let (q0,Rm) = DIVMOD_2EXP 4 opnd2 in
+       let (q1,Sh) = DIVMOD_2EXP 2 (DIV2 q0) in
+       let shift = MOD_2EXP 5 q1 in
+       let rm = REG_READ reg mode (n2w Rm) in
+         SHIFT_IMMEDIATE2 (n2w shift) (n2w Sh) rm C`,
+  ONCE_REWRITE_TAC (map (w2w_n2w_sizes ``:12``) [``:8``, ``:4``, ``:2``])
+    \\ DECODE_TAC);
+
+val SHIFT_REGISTER_THM = store_thm("SHIFT_REGISTER_THM",
+  `!reg mode C opnd2.
+     SHIFT_REGISTER reg mode C (n2w opnd2) =
+       let (q0,Rm) = DIVMOD_2EXP 4 opnd2 in
+       let (q1,Sh) = DIVMOD_2EXP 2 (DIV2 q0) in
+       let Rs = MOD_2EXP 4 (DIV2 q1) in
+       let shift = MOD_2EXP 8 (w2n (REG_READ reg mode (n2w Rs)))
+       and rm = REG_READ (INC_PC reg) mode (n2w Rm) in
+         SHIFT_REGISTER2 (n2w shift) (n2w Sh) rm C`,
+  ONCE_REWRITE_TAC [w2w_n2w_sizes ``:32`` ``:8``]
+    \\ ONCE_REWRITE_TAC (map (w2w_n2w_sizes ``:12``) [``:8``, ``:4``, ``:2``])
+    \\ SIMP_TAC std_ss [SHIFT_REGISTER_def,word_extract_def,
+         (GSYM o SIMP_RULE (std_ss++wordsLib.SIZES_ss) [n2w_w2n,BITS_THM,DIV_1,
+            (GSYM o SIMP_RULE std_ss [] o SPEC `8`) MOD_2EXP_def] o
+          SPECL [`7`,`0`,`w2n (a:word32)`] o
+          Thm.INST_TYPE [alpha |-> ``:32``]) word_bits_n2w]
+    \\ SIMP_TAC word_ss []);
+
+(* ------------------------------------------------------------------------- *)
+
+val REGISTER_LIST_THM = store_thm("REGISTER_LIST_THM",
+  `!n. REGISTER_LIST (n2w n) =
+       let (q0,b0) = DIVMOD_2EXP 1 n in
+       let (q1,b1) = DIVMOD_2EXP 1 q0 in
+       let (q2,b2) = DIVMOD_2EXP 1 q1 in
+       let (q3,b3) = DIVMOD_2EXP 1 q2 in
+       let (q4,b4) = DIVMOD_2EXP 1 q3 in
+       let (q5,b5) = DIVMOD_2EXP 1 q4 in
+       let (q6,b6) = DIVMOD_2EXP 1 q5 in
+       let (q7,b7) = DIVMOD_2EXP 1 q6 in
+       let (q8,b8) = DIVMOD_2EXP 1 q7 in
+       let (q9,b9) = DIVMOD_2EXP 1 q8 in
+       let (q10,b10) = DIVMOD_2EXP 1 q9 in
+       let (q11,b11) = DIVMOD_2EXP 1 q10 in
+       let (q12,b12) = DIVMOD_2EXP 1 q11 in
+       let (q13,b13) = DIVMOD_2EXP 1 q12 in
+       let (q14,b14) = DIVMOD_2EXP 1 q13 in
+       MAP SND (FILTER FST
+         [(b0 = 1,0w); (b1 = 1,1w); (b2 = 1,2w); (b3 = 1,3w);
+          (b4 = 1,4w); (b5 = 1,5w); (b6 = 1,6w); (b7 = 1,7w);
+          (b8 = 1,8w); (b9 = 1,9w); (b10 = 1,10w); (b11 = 1,11w);
+          (b12 = 1,12w); (b13 = 1,13w); (b14 = 1,14w); (ODD q14,15w)])`,
+  DECODE_TAC);
+
+(* ------------------------------------------------------------------------- *)
+
+val DECODE_ARM_THM = store_thm("DECODE_ARM_THM",
+  `!ireg. DECODE_ARM (ireg : word32) =
+    let b n = ireg %% n in
+      if b 27 then
+        if b 26 then
+          if b 25 then
+            if b 24 then (* (T,T,T,T,...) *)
+              swi_ex
+            else (* (T,T,T,F,...) *)
+              if b 4 then
+                if b 20 then mrc else mcr
+              else
+                cdp_und
+          else (* (T,T,F,...) *)
+            ldc_stc
+        else (* (T,F,...) *)
+          if b 25 then br else ldm_stm
+      else
+         if b 26 then (* (F,T,...) *)
+           if b 25 then
+             if b 4 then cdp_und else ldr_str
+           else
+             ldr_str
+         else
+           if b 25 then (* (F,F,T,...) *)
+             if b 24 /\ ~b 23 /\ ~b 20 then
+               if b 21 then
+                 msr
+               else
+                 cdp_und
+             else
+               data_proc
+           else
+             if b 24 then (* (F,F,F,T,...) *)
+               if b 7 then
+                 if b 4 then
+                   if b 20 then
+                     if b 6 then
+                       ldrh_strh
+                     else
+                       if b 5 then
+                         ldrh_strh
+                       else
+                         cdp_und
+                   else
+                     if b 6 then
+                       cdp_und
+                     else
+                       if b 5 then
+                         ldrh_strh
+                       else
+                         if ~b 23 /\ ~b 21 then
+                           swp
+                         else
+                           cdp_und
+                 else
+                   data_proc
+               else
+                 if b 4 then
+                   data_proc
+                 else
+                   if ~b 23 /\ ~b 20 /\ ~b 6 /\ ~b 5 then
+                     if b 21 then msr else mrs
+                   else
+                     data_proc
+             else (* (F,F,F,F,...) *)
+               if b 7 then
+                 if b 4 then
+                   if b 6 \/ b 5 then
+                     if b 20 /\ b 6 then
+                       ldrh_strh
+                     else
+                       if ~b 6 /\ b 5 then
+                         ldrh_strh
+                       else
+                         cdp_und
+                   else
+                     if b 23 \/ ~b 22 then mla_mul else cdp_und
+                 else
+                   data_proc
+               else
+                 if b 4 then data_proc else data_proc`,
+  SRW_TAC [boolSimps.LET_ss] [DECODE_ARM_def]
+    \\ FULL_SIMP_TAC (srw_ss()) [bool_case_ID]);
+
+(*---------------------------------------------------------------------------*)
+
+val num2register = prove(
+  `!n. num2register n =
+         if n = 0 then r0 else
+         if n = 1 then r1 else
+         if n = 2 then r2 else
+         if n = 3 then r3 else
+         if n = 4 then r4 else
+         if n = 5 then r5 else
+         if n = 6 then r6 else
+         if n = 7 then r7 else
+         if n = 8 then r8 else
+         if n = 9 then r9 else
+         if n = 10 then r10 else
+         if n = 11 then r11 else
+         if n = 12 then r12 else
+         if n = 13 then r13 else
+         if n = 14 then r14 else
+         if n = 15 then r15 else
+         if n = 16 then r8_fiq else
+         if n = 17 then r9_fiq else
+         if n = 18 then r10_fiq else
+         if n = 19 then r11_fiq else
+         if n = 20 then r12_fiq else
+         if n = 21 then r13_fiq else
+         if n = 22 then r14_fiq else
+         if n = 23 then r13_irq else
+         if n = 24 then r14_irq else
+         if n = 25 then r13_svc else
+         if n = 26 then r14_svc else
+         if n = 27 then r13_abt else
+         if n = 28 then r14_abt else
+         if n = 29 then r13_und else
+         if n = 30 then r14_und else
+           FAIL num2register ^(mk_var("30 < n",bool)) n`,
+  SRW_TAC [] [num2register_thm, combinTheory.FAIL_THM]);
+
+val num2condition = prove(
+  `!n. num2condition n =
+         if n = 0 then EQ else
+         if n = 1 then CS else
+         if n = 2 then MI else
+         if n = 3 then VS else
+         if n = 4 then HI else
+         if n = 5 then GE else
+         if n = 6 then GT else
+         if n = 7 then AL else
+         if n = 8 then NE else
+         if n = 9 then CC else
+         if n = 10 then PL else
+         if n = 11 then VC else
+         if n = 12 then LS else
+         if n = 13 then LT else
+         if n = 14 then LE else
+         if n = 15 then NV else
+           FAIL num2condition ^(mk_var("15 < n",bool)) n`,
+  SRW_TAC [] [num2condition_thm, combinTheory.FAIL_THM]);
+
+(*---------------------------------------------------------------------------*)
+
+val LDR_STR_OUT = prove(
+  `!r C mode ireg.
+    (LDR_STR r C mode ARB ARB ireg).out =
+      (let (I,P,U,B,W,L,Rn,Rd,offset) = DECODE_LDR_STR ireg in
+       let (addr,wb_addr) = ADDR_MODE2 r.reg mode C I P U Rn offset in
+       let pc_reg = INC_PC r.reg
+       in
+         [(if L then
+             MemRead addr
+           else
+             let w = REG_READ pc_reg mode Rd in
+               MemWrite addr (if B then Byte ((7 >< 0) w) else Word w))])`,
+  SRW_TAC [boolSimps.LET_ss] [LDR_STR_def,DECODE_LDR_STR_def,ADDR_MODE2_def]);
+
+val LDRH_STRH_OUT = prove(
+  `!r C mode ireg.
+    (LDRH_STRH r mode ARB ARB ireg).out =
+      (let (P,U,I,W,L,Rn,Rd,offsetH,S,H,offsetL) = DECODE_LDRH_STRH ireg in
+       let (addr,wb_addr) = ADDR_MODE3 r.reg mode I P U Rn offsetH offsetL in
+       let pc_reg = INC_PC r.reg
+       in
+         [(if L then
+             MemRead addr
+           else
+             MemWrite addr (Half ((15 >< 0) (REG_READ pc_reg mode Rd))))])`,
+  SRW_TAC [boolSimps.LET_ss]
+    [LDRH_STRH_def,DECODE_LDRH_STRH_def,ADDR_MODE3_def]);
+
+val LDM_STM_OUT = prove(
+   `!r mode ireg.
+     (LDM_STM r mode ARB ARB ireg).out =
+       (let (P,U,S,W,L,Rn,list) = DECODE_LDM_STM ireg in
+        let pc_in_list = list %% 15 and rn = REG_READ r.reg mode Rn in
+        let (rp_list,addr_list,rn') = ADDR_MODE4 P U rn list and
+            mode' = (if S /\ (L ==> ~pc_in_list) then usr else mode) and
+            pc_reg = INC_PC r.reg
+        in
+        let wb_reg =
+              (if W /\ ~(Rn = 15w) then
+                 REG_WRITE pc_reg (if L then mode else mode') Rn rn'
+               else
+                 pc_reg)
+        in
+          (if L then
+             MAP MemRead addr_list
+           else
+             STM_LIST (if HD rp_list = Rn then pc_reg else wb_reg)
+               mode' (ZIP (rp_list,addr_list))))`,
+  SRW_TAC [boolSimps.LET_ss] [LDM_STM_def,DECODE_LDM_STM_def,ADDR_MODE4_def]);
+
+val SWP_OUT = prove(
+  `!r mode ireg.
+    (SWP r mode ARB ARB ireg).out =
+       (let (B,Rn,Rd,Rm) = DECODE_SWP ireg in
+        let rn = REG_READ r.reg mode Rn and pc_reg = INC_PC r.reg in
+        let rm = REG_READ pc_reg mode Rm in
+          [MemRead rn;
+           MemWrite rn (if B then Byte ((7 >< 0) rm) else Word rm)])`,
+  SRW_TAC [boolSimps.LET_ss] [SWP_def,DECODE_SWP_def]);
+
+val OUT_ARM =
+   REWRITE_RULE [LDR_STR_OUT,LDRH_STRH_OUT,LDM_STM_OUT,SWP_OUT] OUT_ARM_def;
+
+(*---------------------------------------------------------------------------*)
+
+val register_decl = `register =
+ r0     | r1     | r2      | r3      | r4      | r5      | r6      | r7  |
+ r8     | r9     | r10     | r11     | r12     | r13     | r14     | r15 |
+ r8_fiq | r9_fiq | r10_fiq | r11_fiq | r12_fiq | r13_fiq | r14_fiq |
+                                                 r13_irq | r14_irq |
+                                                 r13_svc | r14_svc |
+                                                 r13_abt | r14_abt |
+                                                 r13_und | r14_und`;
+
+val cp_register_decl = `cp_register =
+   c0 | c1 | c2  | c3  | c4  | c5  | c6  | c7 |
+   c8 | c9 | c10 | c11 | c12 | c13 | c14 | c15`;
+
+val psr_decl =
+  `psr = CPSR | SPSR_fiq | SPSR_irq | SPSR_svc | SPSR_abt | SPSR_und`;
+
+val exceptions_decl = `exceptions = reset | undefined | software | pabort |
+                                    dabort | address |interrupt | fast`;
+
+val mode_decl = `mode = usr | fiq | irq | svc | abt | und | sys | safe`;
+
+val condition_decl = `condition = EQ | CS | MI | VS | HI | GE | GT | AL |
+                                  NE | CC | PL | VC | LS | LT | LE | NV`;
+
+val iclass_decl = `iclass = swp | mrs | msr | data_proc | mla_mul |
+                            ldr_str | ldrh_strh | ldm_stm | br | swi_ex |
+                            cdp_und | mcr | mrc | ldc_stc | unexec`;
+
+val RHS_REWRITE_RULE =
+  GEN_REWRITE_RULE (DEPTH_CONV o RAND_CONV) empty_rewrites;
+
+val n2w_w2n_rule = GEN_ALL o SIMP_RULE bool_ss [wordsTheory.n2w_w2n];
+
+val spec_word_rule16 = n2w_w2n_rule o Q.SPEC `w2n (w:word16)`;
+val spec_word_rule32 = n2w_w2n_rule o Q.SPEC `w2n (w:word32)`;
+
+val spec_word_rule12 =
+  n2w_w2n_rule o INST [`opnd2` |-> `w2n (w:word12)`] o SPEC_ALL;
+
+val mem_read_rule = ONCE_REWRITE_RULE [GSYM mem_read_def];
+
+val _ = ConstMapML.insert ``dimword``;
+val _ = ConstMapML.insert ``dimindex``;
+val _ = ConstMapML.insert ``INT_MIN``;
+val _ = ConstMapML.insert ``n2w_itself``;
+
+fun mk_word n =
+  let val s = Int.toString n
+      val w = "type word" ^ s ^ " = wordsML.word" ^ s
+  in
+    EmitML.MLSIG w
+  end;
+
+val defs_rule =
+  BETA_RULE o PURE_REWRITE_RULE
+    [GSYM n2w_itself_def, GSYM w2w_itself_def, GSYM sw2sw_itself_def,
+     GSYM word_concat_itself_def, GSYM word_extract_itself_def,
+     GSYM mem_write_def, literal_case_THM] o
+  RHS_REWRITE_RULE [GSYM word_eq_def];
+
+val _ = let open EmitML in emitML (!Globals.emitMLDir)
+    ("bsubst", OPEN ["num", "fcp", "words"]
+         :: MLSIG "type 'a word = 'a wordsML.word"
+         :: MLSIG "type num = numML.num"
+         :: MLSIG "type word2 = wordsML.word2"
+         :: MLSIG "type word8 = wordsML.word8"
+         :: MLSIG "type word16 = wordsML.word16"
+         :: MLSIG "type word30 = wordsML.word30"
+         :: MLSIG "type word32 = wordsML.word32"
+         :: MLSTRUCT "type mem = word30->word32"
+         :: MLSIG "type mem"
+         :: MLSTRUCT "val mem_updates = ref ([]: word30 list)"
+         :: MLSIG "val mem_updates : word30 list ref"
+         :: DATATYPE (`formats = SignedByte | UnsignedByte
+                               | SignedHalfWord | UnsignedHalfWord
+                               | UnsignedWord`)
+         :: DATATYPE (`data = Byte of word8 | Half of word16 | Word of word32`)
+         :: map DEFN
+              [SUBST_def, BSUBST_def, mem_read_def,
+               mem_write_def, mem_write_block_def]
+          @ map (DEFN o defs_rule o ONCE_REWRITE_RULE [GSYM mem_read_def])
+              [empty_memory_def, mem_items_def, ADDR30_def, GET_HALF_def,
+               SIMP_RULE std_ss [literal_case_DEF] GET_BYTE_def,
+               FORMAT_def, SET_BYTE_def, SET_HALF_def,
+               MEM_WRITE_BYTE_def, MEM_WRITE_HALF_def,
+               MEM_WRITE_WORD_def, MEM_WRITE_def])
+end;
+
+val _ = temp_type_abbrev("cp_registers32",``:32 cp_registers``);
+
+val _ = let open EmitML in emitML (!Globals.emitMLDir) ("arm",
+  OPEN ["num", "option", "set", "fcp", "list", "rich_list", "bit", "words"]
+    :: MLSIG "type 'a word = 'a wordsML.word"
+    :: MLSIG "type num = numML.num"
+    :: map (fn decl => DATATYPE decl) [register_decl, cp_register_decl,
+                                       psr_decl, mode_decl, condition_decl]
+     @ map (fn decl => EQDATATYPE ([], decl)) [exceptions_decl,iclass_decl]
+     @ ABSDATATYPE (["'a","'b"],`state_inp = <| state : 'a; inp : num -> 'b |>`)
+    :: ABSDATATYPE (["'a","'b"],`state_out = <| state : 'a; out : 'b |>`)
+    :: map mk_word [2,4,5,8,12,16,24,30,32]
+     @ MLSTRUCT "type registers = register->word32"
+    :: MLSTRUCT "type 'a cp_registers = cp_register->'a word"
+    :: MLSTRUCT "type cp_registers32 = cp_register-> word32"
+    :: MLSTRUCT "type psrs = psr->word32"
+    :: MLSTRUCT "type mem = bsubstML.mem"
+    :: MLSTRUCT "type data = bsubstML.data"
+    :: MLSIG "type registers = register->word32"
+    :: MLSIG "type 'a cp_registers = cp_register->'a word"
+    :: MLSIG "type cp_registers32 = cp_register-> word32"
+    :: MLSIG "type psrs = psr->word32"
+    :: MLSIG "type mem = bsubstML.mem"
+    :: MLSIG "type data = bsubstML.data"
+    :: DATATYPE (`all_cp_registers = <|
+            p0_registers:'a0 cp_registers; p1_registers:'a1 cp_registers;
+            p2_registers:'a2 cp_registers; p3_registers:'a3 cp_registers;
+            p4_registers:'a4 cp_registers; p5_registers:'a5 cp_registers;
+            p6_registers:'a6 cp_registers; p7_registers:'a7 cp_registers;
+            p8_registers:'a8 cp_registers; p9_registers:'a9 cp_registers;
+            p10_registers:'a10 cp_registers; p11_registers:'a11 cp_registers;
+            p12_registers:'a12 cp_registers; p13_registers:'a13 cp_registers;
+            p14_registers:'a14 cp_registers; p15_registers:32 cp_registers
+          |>`)
+    :: DATATYPE (`regs = <| reg : registers; psr : psrs |>`)
+    :: DATATYPE (`memop = MemRead of word32 | MemWrite of word32=>data |
+                          CPWrite of word32`)
+    :: DATATYPE (`arm_state = <| regs : regs; ireg : word32;
+                                 exception : exceptions |>`)
+    :: DATATYPE (`arm_output = <| transfers : memop list;
+                                  cpi : bool; user : bool |>`)
+    :: DATATYPE (`cp_output = <| data : word32 option list; absent : bool |>`)
+    :: DATATYPE (`bus = <| data : word32 list; memory : mem; abort : num option;
+                           p15_registers : 32 cp_registers |>`)
+    :: DATATYPE (`arm_sys_state = <| registers : registers; psrs : psrs;
+            memory : mem; undefined : bool;
+            cp_registers : ('a0,'a1,'a2,'a3,'a4,'a5,'a6,'a7, 'a8,'a9,
+                            'a10,'a11,'a12,'a13,'a14) all_cp_registers |>`)
+    :: DATATYPE (`interrupt = Reset of regs | Undef | Prefetch |
+                              Dabort of num | Fiq | Irq`)
+    :: DATATYPE (`arm_input = <| ireg : word32; data : word32 list;
+                                 interrupt : interrupt option; no_cp : bool |>`)
+    :: MLSTRUCT "val mem_updates = ref ([]: word30 list)"
+    :: MLSIG "val mem_updates : word30 list ref"
+    :: map (DEFN o defs_rule) (map spec_word_rule32
+         [DECODE_PSR_THM, DECODE_BRANCH_THM, DECODE_DATAP_THM,
+          DECODE_MRS_THM, DECODE_MSR_THM, DECODE_LDR_STR_THM,
+           DECODE_MLA_MUL_THM, DECODE_LDM_STM_THM, DECODE_SWP_THM,
+           DECODE_LDC_STC_THM, DECODE_LDRH_STRH_THM]
+       @ [USER_def, mode_reg2num_def, DECODE_ARM_def, mode_num_def,
+          state_out_state, state_out_out, exceptions2num_thm, register2num_thm,
+          num2register, num2condition, SET_IFMODE_def,
+          REG_READ_def, REG_WRITE_def, INC_PC_def, FETCH_PC_def,
+          SET_NZCV_def, SET_NZC_def, SET_NZ_def,
+          SIMP_RULE std_ss [literal_case_DEF] DECODE_MODE_def,
+          NZCV_def, CARRY_def, mode2psr_def, SPSR_READ_def, CPSR_READ_def,
+          CPSR_WRITE_def, SPSR_WRITE_def, exception2mode_def,
+          SPECL [`r`,`e`]  EXCEPTION_def, BRANCH_def, LSL_def, LSR_def,
+          ASR_def, ROR_def, IMMEDIATE_def, SHIFT_IMMEDIATE2_def,
+          SHIFT_REGISTER2_def, spec_word_rule12 SHIFT_IMMEDIATE_THM,
+          spec_word_rule12 SHIFT_REGISTER_THM, ADDR_MODE1_def,
+          SPEC `f` ALU_arith_def, SPEC `f` ALU_arith_neg_def, ALU_logic_def,
+          numLib.REDUCE_RULE SUB_def, ADD_def, AND_def, EOR_def, ORR_def,
+          ALU_def, ARITHMETIC_def, TEST_OR_COMP_def, DATA_PROCESSING_def,
+          MRS_def, MSR_def, ALU_multiply_def, MLA_MUL_def,
+          UP_DOWN_def, ADDR_MODE2_def, IMP_DISJ_THM, LDR_STR_def,
+          ADDR_MODE3_def, LDRH_STRH_def,spec_word_rule16 REGISTER_LIST_THM,
+          ADDRESS_LIST_def, WB_ADDRESS_def, FIRST_ADDRESS_def,
+          ADDR_MODE4_def, LDM_LIST_def, STM_LIST_def, LDM_STM_def,
+          SWP_def, MRC_def, MCR_OUT_def, ADDR_MODE5_def, LDC_STC_def,
+          CONDITION_PASSED2_def, CONDITION_PASSED_def,
+          RUN_ARM_def, IS_Reset_def, PROJ_Dabort_def, PROJ_Reset_def ,
+          interrupt2exception_def, PROJ_IF_FLAGS_def, NEXT_ARM_def,
+          OUT_ARM, mem_read_rule TRANSFER_def, TRANSFERS_def,
+          mem_read_rule NEXT_ARM_MEM, empty_registers_def,
+          empty_cp_registers_def, empty_all_cp_registers_def]))
+ end;
+
+(* -------------------------------------------------------------------------- *)
+
+val _ = export_theory();
